Seccap/AlphaEquiv.lean
@@ -1,0 +1,70 @@
+import Seccap.Basic
+import Seccap.Finmap
+
+inductive CExpr.DeBruijn where
+| unit
+| nat (n: ℕ)
+| bvar (n: ℕ)
+| fvar (x: Var)
+| abs (e: DeBruijn)
+| app (e₁ e₂ : DeBruijn)
+| comp (e₁ e₂ : DeBruijn)
+| setb (n : ℕ) (e : DeBruijn)
+| setf (x: Var) (e: DeBruijn)
+
+namespace CExpr.DeBruijn
+def fvs : DeBruijn → Finset Var
+| fvar x => {x}
+| abs e => e.fvs
+| app e₁ e₂ | comp e₁ e₂ => e₁.fvs ∪ e₂.fvs
+| setf x e => {x} ∪ e.fvs
+| _ => ∅
+
+def fromExpr (e: CExpr) : DeBruijn :=
+  helper 0 0 (by simp) e
+  where helper (Γ: Finmap Var ℕ) (d : ℕ) (hΓ : ∀ x, (h : x ∈ Γ.support) → Γ.get x h < d): CExpr → DeBruijn
+  | .unit => .unit
+  | .nat n => .nat n
+  | .var x => match Γ x with
+    | some n => .bvar n
+    | none => .fvar x
+  | .abs x e => helper (Finmap.insert (Finsupp.mk
+    Γ.support
+    (Γ · |>.map (· + 1))
+    (by
+      intro a
+      rw [Finmap.mem_support_is_some]
+      constructor
+      · intro h
+        simp
+        apply Option.isSome_iff_exists.mp at h
+        have ⟨a, ha⟩ := h
+        rw [ha]
+        simp
+      · intro h
+        simp [OfNat.ofNat, Zero.zero] at h
+        exact Option.isSome_iff_ne_none.mpr h
+    )
+  ) x 0) (d + 1) (by
+    simp
+    intro x' h
+    simp [Finmap.insert, Finmap.get]
+    cases h with
+    | inl h =>
+      subst h
+      simp
+    | inr h =>
+      split_ifs
+      · simp
+      · simp
+        apply hΓ
+        exact Finsupp.mem_support_iff.mpr h
+  ) e
+  | .set x e =>
+    let e' := helper Γ d hΓ e
+    match Γ x with
+    | some n => .setb n e'
+    | none => .setf x e'
+  | .app e₁ e₂ => .app (helper Γ d hΓ e₁) (helper Γ d hΓ e₂)
+  | .comp e₁ e₂ => .comp (helper Γ d hΓ e₁) (helper Γ d hΓ e₂)
+end DeBruijn
