Seccap/Nominal.lean
@@ -1,0 +1,557 @@
+import Std.Data.ExtTreeMap.Basic
+import Std.Data.ExtTreeMap.Lemmas
+import Mathlib.Data.Finset.Basic
+import Mathlib.Data.Fintype.EquivFin
+import Mathlib.Data.Finite.Defs
+
+variable {𝔸 : Type} [DecidableEq 𝔸]
+
+inductive Perm 𝔸 where
+| id
+| prod (π: Perm 𝔸) (a b : 𝔸) (h: a ≠ b)
+
+
+def transpose (a b : 𝔸) : 𝔸 → 𝔸  :=
+  fun x => if x = a then b else if x = b then a else x
+
+lemma transpose_involutive (a b: 𝔸): Function.Involutive (transpose a b) := by
+  intro x
+  simp [transpose]
+  aesop
+
+@[simp]
+lemma transpose_a (a b : 𝔸): (transpose a b) a = b := by simp [transpose]
+
+@[simp]
+lemma transpose_b (a b : 𝔸): (transpose a b) b = a := by simp [transpose]
+
+def Perm.toEquiv : Perm 𝔸 → Equiv.Perm 𝔸
+| id => {
+    toFun := _root_.id
+    invFun := _root_.id
+  }
+| prod π a b h => {
+    toFun := π.toEquiv ∘ transpose a b
+    invFun := transpose a b ∘ π.toEquiv.symm
+    left_inv := by
+      intro x
+      simp
+      apply transpose_involutive
+    right_inv := by
+      intro x
+      simp
+      rw [transpose_involutive]
+      simp
+  }
+
+@[ext]
+axiom perm_ext (π₁ π₂ : Perm 𝔸):
+  π₁.toEquiv = π₂.toEquiv → π₁ = π₂
+
+instance : EquivLike (Perm 𝔸) 𝔸 𝔸 where
+  coe := (·.toEquiv)
+  inv := (·.toEquiv.symm)
+  left_inv := (·.toEquiv.left_inv)
+  right_inv := (·.toEquiv.right_inv)
+  coe_injective' := by
+    intro x y ha hb
+    ext a
+    rw [ha]
+
+
+
+
+@[simp]
+lemma Perm.coe_eq (π: Perm 𝔸) (a: 𝔸) :
+  π a = π.toEquiv.toFun a := rfl
+
+
+def Perm.vars : Perm 𝔸 → Finset 𝔸
+| id => ∅
+| prod π a b _ => π.vars ∪ {a, b}
+
+def Perm.support (π: Perm 𝔸) : Finset 𝔸 :=
+  {x ∈ π.vars | π x ≠ x}
+
+lemma Perm.support_iff (π : Perm 𝔸) :
+  ∀ x, x ∈ π.support ↔ π x ≠ x := by
+  intro x
+  constructor
+  · simp [support]
+  · intro hx
+    induction π generalizing x with
+    | id => absurd hx; rfl
+    | prod π a b h ih =>
+      simp [] at hx
+      by_cases ha: x = a
+      · subst ha
+        simp [toEquiv, transpose] at hx
+        simp [support, toEquiv, vars, transpose]
+        exact hx
+      · by_cases hb: x = b
+        · subst hb
+          simp [toEquiv] at hx
+          simp [support, vars, toEquiv, hx]
+        · simp [support, vars, toEquiv, ha, hb, transpose]
+          simp [toEquiv, transpose, ha, hb] at hx
+          constructor
+          · specialize ih x hx
+            simp [support] at ih
+            exact ih.left
+          · exact hx
+
+def Perm.difference_set (π₁ π₂ : Perm 𝔸) :=
+  {a ∈ π₁.support ∪ π₂.support | π₁ a ≠ π₂ a}
+
+infix:80 "∆"  => Perm.difference_set
+
+lemma Perm.difference_set_iff (π₁ π₂ : Perm 𝔸):
+  ∀ a, a ∈ π₁ ∆ π₂ ↔ π₁ a ≠ π₂ a := by
+  intro a
+  simp [difference_set]
+  intro h
+  by_cases h': π₁ a = a
+  · right
+    rw [support_iff]
+    intro c
+    apply h
+    simp at h'
+    simp at c
+    rw [h', c]
+  · left
+    rw [support_iff]
+    exact h'
+
+
+lemma Perm.difference_set_refl (π : Perm 𝔸) : π ∆ π = ∅ :=
+  by simp [difference_set]
+
+lemma Perm.difference_set_symm (π₁ π₂ : Perm 𝔸) :
+  π₁ ∆ π₂ = π₂ ∆ π₁ := by
+  ext a
+  simp [difference_set_iff]
+  tauto
+
+theorem Perm.difference_set_triangle (π₁ π₂ π₃ : Perm 𝔸) :
+    π₁ ∆ π₃ ⊆ π₁ ∆ π₂ ∪ π₂ ∆ π₃ := by
+  intro a ha
+  rw [Perm.difference_set_iff] at ha
+  simp [Finset.mem_union, Perm.difference_set_iff, Perm.difference_set_iff]
+  by_cases h: (π₁ a = π₂ a)
+  · right; exact h ▸ ha
+  · left; exact h
+
+
+def Perm.comp (π₁ : Perm 𝔸) : Perm 𝔸 → Perm 𝔸
+| id => π₁
+| prod π₂ a b h => (π₁.comp π₂).prod a b h
+
+infix:70 " ∘ₚ " => Perm.comp
+
+
+omit [DecidableEq 𝔸] in
+@[simp]
+lemma Perm.id_comp (π : Perm 𝔸) : id ∘ₚ π = π := by
+  induction π with
+  | id => simp [comp]
+  | prod π a b h ih => simp [comp, ih]
+
+lemma Perm.comp_coe (π₁ π₂ : Perm 𝔸): (π₁ ∘ₚ π₂).toEquiv = π₁.toEquiv ∘ π₂.toEquiv := by
+  induction π₂ generalizing π₁ with
+  | id => simp [comp, toEquiv]
+  | prod π a b h ih =>
+    simp [comp, toEquiv, ih, Function.comp_assoc]
+
+lemma Perm.comp_assoc (π₁ π₂ π₃ : Perm 𝔸) :
+  (π₁ ∘ₚ π₂) ∘ₚ π₃ = π₁ ∘ₚ (π₂ ∘ₚ π₃) := by
+  ext x
+  simp [comp_coe]
+
+def Perm.inv : Perm 𝔸 → Perm 𝔸
+| id => id
+| prod π a b h => (id.prod a b h) ∘ₚ π.inv
+
+@[simp]
+lemma Perm.inv_toEquiv (π : Perm 𝔸):
+  π.inv.toEquiv = π.toEquiv.symm := by
+  ext x
+  induction π with simp [inv, toEquiv, comp_coe, *]
+
+variable {𝔸 𝕏 C: Type} [DecidableEq 𝔸]
+inductive Term 𝔸 𝕏 C where
+| atom (a: 𝔸)
+| unknown (π: Perm 𝔸) (X: 𝕏)
+| abs (a: 𝔸) (t: Term 𝔸 𝕏 C)
+| app (t₁ t₂: Term 𝔸 𝕏 C)
+| const (c: C)
+
+namespace Term
+
+abbrev unknown' (X: 𝕏) : Term 𝔸 𝕏 C :=
+  unknown .id X
+
+def atoms : Term 𝔸 𝕏 C → Finset 𝔸
+| atom a => {a}
+| unknown π _ => π.support
+| abs a t => {a} ∪ t.atoms
+| app t₁ t₂ => t₁.atoms ∪ t₂.atoms
+| const _ => ∅
+
+def perm_action (π: Perm 𝔸) : Term 𝔸 𝕏 C → Term 𝔸 𝕏 C
+| atom a => atom (π a)
+| unknown π' X => unknown (π ∘ₚ π') X
+| abs a t =>  abs (π a) (t.perm_action π)
+| app t₁ t₂ => app (t₁.perm_action π) (t₂.perm_action π)
+| const c => const c
+
+infix:80 " · " => perm_action
+
+def subst (σ : 𝕏 → Term 𝔸 𝕏 C) : Term 𝔸 𝕏 C → Term 𝔸 𝕏 C
+| atom a => atom a
+| unknown π X => π · (σ X)
+| abs a t => abs a (t.subst σ)
+| app t₁ t₂ => app (t₁.subst σ) (t₂.subst σ)
+| const c => const c
+
+abbrev FreshnessCtx 𝔸 𝕏 := Finset (𝔸 × 𝕏)
+
+inductive Fresh (Δ : FreshnessCtx 𝔸 𝕏): 𝔸 → Term 𝔸 𝕏 C → Prop where
+| F_hyp a X : (a, X) ∈ Δ → Fresh Δ a (unknown' X)
+| F_atom (a b : 𝔸) (h: a ≠ b): Fresh Δ a (atom b)
+| F_unknown a π X : Fresh Δ (π.toEquiv.symm a) (unknown' X) → Fresh Δ a (unknown π X)
+| F_absa a t : Fresh Δ a (abs a t)
+| F_absb a b t (h: a ≠ b) : Fresh Δ a t → Fresh Δ a (abs b t)
+| F_app a t₁ t₂ : Fresh Δ a t₁ → Fresh Δ a t₂ → Fresh Δ a (app t₁ t₂)
+| F_const a c : Fresh Δ a (const c)
+
+notation:50 Δ:50 " ⊢ " a:50 " # " t:50 => Term.Fresh Δ a t
+
+namespace Fresh
+
+lemma weakening Δ Γ a (t: Term 𝔸 𝕏 C) : Δ ⊢ a#t → Δ ⊆ Γ → Γ ⊢ a#t := by
+  intro hf hΔ
+  induction hf with constructor <;> try assumption
+  | F_hyp a X h => exact hΔ h
+
+end Fresh
+
+
+abbrev Theory := Finset (FreshnessCtx 𝔸 𝕏 × Term 𝔸 𝕏 C × Term 𝔸 𝕏 C)
+
+inductive NominalEq (T: Theory) (Δ: FreshnessCtx 𝔸 𝕏) : Term 𝔸 𝕏 C → Term 𝔸 𝕏 C → Prop where
+| N_refl t : NominalEq T Δ t t
+| N_symm t u : NominalEq T Δ t u → NominalEq T Δ u t
+| N_trans t u v : NominalEq T Δ t u → NominalEq T Δ u v → NominalEq T Δ t v
+| N_perm a b t (h: a ≠ b) : (Δ ⊢ a#t) → (Δ ⊢ b#t) → NominalEq T Δ ((.prod .id a b h)·t) t
+| N_cngAbs a t u : NominalEq T Δ t u → NominalEq T Δ (abs a t) (abs a u)
+| N_cngApp t₁ t₂ u₁ u₂ : NominalEq T Δ t₁ u₁ → NominalEq T Δ t₂ u₂ → NominalEq T Δ (app t₁ t₂) (app u₁ u₂)
+| N_ax Γ t u π σ : (Γ, t, u) ∈ T → ∀ p ∈ Γ, (Δ ⊢ p.fst # (unknown' p.snd).subst σ) →
+  NominalEq T Δ (π ·(t.subst σ)) (π ·(u.subst σ))
+
+namespace NominalEq
+
+lemma equiv {T: @Theory 𝔸 𝕏 C} {Δ}: Equivalence (Term.NominalEq T Δ) where
+  refl := N_refl
+  symm := by apply N_symm
+  trans := by apply N_trans
+
+end NominalEq
+
+
+def ground : Term 𝔸 𝕏 C → Bool
+| atom _ | const _ => true
+| unknown _ _ => false
+| abs _ t => t.ground
+| app t₁ t₂ => t₁.ground ∧ t₂.ground
+
+abbrev CoreEq := @NominalEq 𝔸 𝕏 C _ ∅
+
+-- inductive Term.CoreEq' (Δ : FreshnessCtx 𝔸 𝕏) : Term 𝔸 𝕏 C → Term 𝔸 𝕏 C → Prop where
+-- | C_atom a : CoreEq' Δ (atom a) (atom a)
+-- | C_unknown π₁ π₂ X : (∀ a ∈ π₁∆π₂, Term.Fresh (C := C) Δ a (unknown' X)) →
+--   CoreEq' Δ (unknown π₁ X) (unknown π₂ X)
+-- | C_absa a t u : CoreEq' Δ t u → CoreEq' Δ (abs a t) (abs a u)
+-- | C_absb a b (h: a ≠ b) t u : Δ ⊢ b#t → CoreEq' Δ ((.prod .id a b h)·t) u →
+--   CoreEq' Δ (abs a t) (abs b u)
+-- | C_app t₁ t₂ u₁ u₂ : CoreEq' Δ t₁ u₁ → CoreEq' Δ t₂ u₂ →
+--   CoreEq' Δ (app t₁ t₂) (app u₁ u₂)
+-- | C_const c : CoreEq' Δ (const c) (const c)
+
+
+lemma ground_notin_atoms (t: Term 𝔸 𝕏 C) a (hg: t.ground):
+  a ∉ t.atoms → ∅ ⊢ a#t := by
+  intro h
+  induction t with simp [atoms] at h
+  | atom b => apply Fresh.F_atom; assumption
+  | unknown π x => simp [ground] at hg
+  | abs x t ih =>
+    simp [ground] at hg
+    apply Fresh.F_absb
+    exact h.left
+    exact ih hg h.right
+  | app t₁ t₂ ih₁ ih₂ =>
+    simp [ground] at hg
+    apply Fresh.F_app
+    apply ih₁
+    exact hg.left
+    exact h.left
+    apply ih₂
+    exact hg.right
+    exact h.right
+  | const => apply Fresh.F_const
+
+lemma ex_fresh' [Infinite 𝔸] (t: Term 𝔸 𝕏 C) :
+  ∃ a, a ∉ t.atoms := Infinite.exists_notMem_finset t.atoms
+
+lemma ex_fresh [Infinite 𝔸] (t: Term 𝔸 𝕏 C) (hg: t.ground):
+  ∃ a, ∅ ⊢ a#t := by
+  obtain ⟨a, ha⟩: ∃ a, a ∉ t.atoms := Infinite.exists_notMem_finset t.atoms
+  use a
+  apply ground_notin_atoms <;> assumption
+
+
+lemma perm_action_ground (t: Term 𝔸 𝕏 C) π :
+  (π·t).ground = t.ground := by
+  induction t with simp [Term.perm_action, ground]
+  | abs a t ih => exact ih
+  | app t₁ t₂ ih₁ ih₂ => simp [ih₁, ih₂]
+
+inductive GroundDeBruijn (𝔸 C) where
+| bvar (n: ℕ)
+| fvar (a: 𝔸)
+| const (c: C)
+| abs (t: GroundDeBruijn 𝔸 C)
+| app (t₁ t₂ : GroundDeBruijn 𝔸 C)
+
+namespace GroundDeBruijn
+-- permute f vars
+def perm_action (π : Perm 𝔸) : GroundDeBruijn 𝔸 C → GroundDeBruijn 𝔸 C
+| fvar a => fvar (π a)
+| abs t => abs (t.perm_action π)
+| app t₁ t₂ => app (t₁.perm_action π) (t₂.perm_action π)
+| t => t
+end GroundDeBruijn
+
+def debruijnify (t: Term 𝔸 𝕏 C) (ht: t.ground) : GroundDeBruijn 𝔸 C :=
+  go {} t ht
+  where go (l: List 𝔸) t (ht: t.ground) := match t with
+  | const c => .const c
+  | atom a => match l.idxOf? a with
+    | some n => .bvar n
+    | none => .fvar a
+  | unknown .. => by simp [ground] at ht
+  | abs a t => .abs <| go (a :: l) t (by simp [ground] at ht; exact ht)
+  | app t₁ t₂ =>
+    .app (go l t₁ (by simp [ground] at ht; exact ht.left))  (go l t₂ (by simp [ground] at ht; exact ht.right))
+
+abbrev swap (t: Term 𝔸 𝕏 C) a b (h: a ≠ b):=
+  (Perm.id.prod a b h)·t
+
+lemma swap_fresh (t: Term 𝔸 𝕏 C) a b (h: a ≠ b) Δ (hb: Δ ⊢ b#t) (ht: t.ground):
+  Δ ⊢ a#(t.swap a b h) := by
+  induction t with
+  | atom x =>
+    cases hb
+    expose_names
+    apply Fresh.F_atom
+    simp [Perm.toEquiv]
+    intro c
+    simp [transpose, h_1.symm] at c
+    split_ifs at c with hc
+    · subst hc; contradiction
+    · cases hc c.symm
+  -- todo
+  | unknown π x => simp [ground] at ht
+  | const c => simp [perm_action]; constructor
+  | app t₁ t₂ ih₁ ih₂ =>
+    cases hb
+    expose_names
+    simp [ground] at ht
+    constructor
+    apply ih₁
+    exact h_1
+    exact ht.left
+    apply ih₂
+    exact h_2
+    exact ht.right
+  | abs x t ih =>
+    simp [ground] at ht
+    cases hb with
+    | F_absa =>
+      simp [perm_action, Perm.toEquiv]
+      apply Fresh.F_absa
+    | F_absb _ _ _ hb hf =>
+      apply Fresh.F_absb
+      simp [Perm.toEquiv, transpose, hb.symm]
+      split_ifs with hx
+      · subst hx; assumption
+      · intro c; cases hx c.symm
+      apply ih <;> assumption
+
+lemma perm_debruijn
+  (t: Term 𝔸 𝕏 C) (ht: t.ground) l π:
+    debruijnify.go (l.map (π.inv)) t ht = (debruijnify.go l (π·t) (by simp [perm_action_ground, ht])).perm_action π.inv
+  := by
+  induction t generalizing l π with
+  | atom x =>
+    simp [debruijnify.go, perm_action]
+    induction l with
+    | nil => simp [GroundDeBruijn.perm_action, Perm.inv_toEquiv]
+    | cons a l ih =>
+      cases h: (a == π x) with
+      | true =>
+        simp at h
+        simp [List.idxOf?_cons, h, GroundDeBruijn.perm_action]
+      | false =>
+        simp at h
+        simp [List.idxOf?_cons, h]
+        have : (π.inv a ≠ x) := by
+          intro c
+          rw [← c] at h
+          simp at h
+        simp at this
+        simp [this]
+        simp at ih
+        split at ih <;> split at ih <;> simp [GroundDeBruijn.perm_action] at ih
+        · expose_names
+          simp [heq, heq_1, ih, GroundDeBruijn.perm_action]
+        · expose_names
+          simp [heq, heq_1, GroundDeBruijn.perm_action]
+  | unknown => simp [ground] at ht
+  | abs x t ih =>
+    simp [debruijnify.go, GroundDeBruijn.perm_action, perm_action]
+    simp [ground] at ht
+    rw [← ih]
+    simp
+    exact ht
+  | app t₁ t₂ ih₁ ih₂ =>
+    simp [ground] at ht
+    obtain ⟨ht₁, ht₂⟩ := ht
+    simp [debruijnify.go, GroundDeBruijn.perm_action, perm_action]
+    constructor
+    · simp [ih₁]
+    · simp [ih₂]
+  | const c => simp [perm_action, debruijnify.go, GroundDeBruijn.perm_action]
+
+
+-- Proof that if CoreEq a b, we can find a renaming function to make a = b.
+namespace CoreEq
+lemma coreeq_ground {t₁ t₂ : Term 𝔸 𝕏 C} {Δ} (heq: CoreEq Δ t₁ t₂):
+   t₁.ground = t₂.ground := by
+  induction heq with
+  | N_refl => rfl
+  | N_symm => symm; assumption
+  | N_trans t₁ t₂ t₃ h₁₂ h₂₃ ih₁ ih₂ => simp [ih₁, ih₂]
+  | N_perm a b t h ha hb => apply Term.perm_action_ground
+  | N_cngAbs a t₁ t₂ heq ih => simp [ground, ih]
+  | N_cngApp t₁ t₂ u₁ u₂ heq₁ heq₂ ih₁ ih₂ => simp [ground, ih₁, ih₂]
+  | N_ax _ _ _ _ _ hp => cases hp
+
+
+theorem chain_de_bruijn [Infinite 𝔸] (t₁ t₂: Term 𝔸 𝕏 C) (hg₁: t₁.ground)
+  (ht: Term.CoreEq ∅ t₁ t₂):
+  debruijnify t₁ (hg₁) = debruijnify t₂ (by rw [← coreeq_ground ht]; exact hg₁) := by
+  sorry
+
+
+end CoreEq
+end Term
+
+
+
+
+
+
+
+
+
+
+
+
+
+
+
+
+
+
+
+
+
+
+
+
+-- structure Permutation where
+--   map : 𝔸 → 𝔸
+--   map_bij : Function.Bijective map
+--   support: Finset 𝔸
+--   map_support_iff : ∀ a, a ∈ support ↔ map a ≠ a
+
+-- def Permutation.transposition  [DecidableEq 𝔸] (a b : 𝔸) (h: a ≠ b) : Permutation 𝔸 :=
+--   {
+--     map := fun x => if x = a then b else if x = b then a else x
+--     map_bij := by
+--       constructor
+--       · unfold Function.Injective
+--         aesop
+--       · intro x
+--         by_cases x = b
+--         · use a; aesop
+--         · by_cases x = a
+--           · use b; aesop
+--           · use x; aesop
+--     support := {a, b}
+--     map_support_iff := by aesop
+--   }
+
+-- lemma Permutation.map_inj (π ρ : Permutation 𝔸):
+--   π.map = ρ.map → π = ρ := by
+--   intro h
+--   obtain ⟨f₁, hi₁, sup₁, hs₁⟩ := π
+--   obtain ⟨f₂, hi₂, sup₂, hs₂⟩ := ρ
+--   simp
+--   simp at h
+--   constructor; try assumption
+--   ext x
+--   constructor
+--   · intro h₁
+--     apply (hs₂ x).mpr
+--     rw [← h]
+--     apply (hs₁ x).mp
+--     exact h₁
+--   · intro h₂
+--     apply (hs₁ x).mpr
+--     rw [h]
+--     apply (hs₂ x).mp
+--     exact h₂
+
+
+-- instance : FunLike (Permutation 𝔸) 𝔸 𝔸 where
+--   coe := (·.map)
+--   coe_injective' := by intro a b; simp; apply Permutation.map_inj
+
+-- variable (π : Permutation 𝔸)
+-- lemma Permutation.closed x : x ∈ π.support ↔ π x ∈ π.support := by
+--   constructor
+--   · intro h
+--     by_contra
+--     have := (π.map_support_iff (π x)).mpr
+--     contrapose this
+
+
+
+
+
+-- def Permutation.inverse [DecidableEq 𝔸] (π : Permutation 𝔸): Permutation 𝔸 :=
+--   {
+--     support := π.support
+--     map := fun x => if hx: x ∈ π.support then π.support.choose (fun a ↦ π a = x) (by
+
+--     )  else x
+--   }
+
+-- variable (𝔸 𝕏: Type) [Infinite 𝔸]  [Infinite 𝕏] [DecidableEq 𝔸]
+
+-- inductive Term where
+-- | atom (a : 𝔸)
+-- | unknown (π : Permutation 𝔸) (X : 𝕏)
+-- |
