Seccap/SecTypes.lean
@@ -1,0 +1,34 @@
+import Mathlib.Order.Lattice
+import Seccap.Basic
+
+inductive BType where
+| unit
+| nat
+
+inductive SType L [SemilatticeSup L] where
+| base (b : BType) (l: L)
+| arrow (t1 t2 : SType L) (pc : L)
+
+inductive SExpr L [SemilatticeSup L] where
+| unit
+| nat (n: ℕ)
+| abs (x: Var) (e: SExpr L)
+--- val
+| var (x: Var) (l: L)
+| app (e₁ e₂ : SExpr L)
+| set (x: Var) (e: SExpr L) (l: L)
+| comp (e₁ e₂ : SExpr L)
+
+variable {L} [SemilatticeSup L] (e: SExpr L)
+
+def SExpr.cexpr : SExpr L → CExpr
+| unit => .unit
+| nat n => .nat n
+| abs x e => .abs x e.cexpr
+| var x _ => .var x
+| app e₁ e₂ => .app e₁.cexpr e₂.cexpr
+| set x e _ => .set x e.cexpr
+| comp e₁ e₂ => .comp e₁.cexpr e₂.cexpr
+
+abbrev SExpr.fvs := e.cexpr.fvs
+abbrev SExpr.bvs := e.cexpr.bvs
