Seccap/SimpleTypes.lean
@@ -1,5 +1,6 @@
 import Seccap.Basic
 import Seccap.Finmap
+import Seccap.AlphaEquiv
 
 inductive CType where
 | unit
@@ -11,7 +12,7 @@ inductive CExpr.Type : Finmap Var CType → CExpr → CType → Prop where
 | unit Γ : CExpr.Type Γ .unit .unit
 | nat Γ n : CExpr.Type Γ (.nat n) .nat
 | var Γ x τ (h : Γ x = some τ) : CExpr.Type Γ (.var x) τ
-| abs Γ x e τ₁ τ₂ :
+| abs Γ x e τ₁ τ₂:
   CExpr.Type (Γ.insert x τ₁) e τ₂ →
   CExpr.Type Γ (.abs x e) (.arrow τ₁ τ₂)
 | app Γ e₁ e₂ τ₁ τ₂ : CExpr.Type Γ e₁ (.arrow τ₁ τ₂) →
@@ -42,3 +43,108 @@ lemma CExpr.Type.arrow_canonical Γ (v: CVal) τ₁ τ₂:
   intro ht
   cases v with cases ht
   | abs x e => use x,e
+
+lemma CExpr.Type.weakening Γ e τ Γ':
+  (∀ x ∈ Γ.support, Γ x = Γ' x) →
+  (Γ ⊢ e : τ) →
+  (Γ' ⊢ e : τ) := by
+  intro hΓ hτ
+  induction hτ generalizing Γ' with try (constructor; done)
+  | var Γ x τ h =>
+    constructor
+    rw [← hΓ]
+    assumption
+    apply (Γ.mem_support_is_some x).mpr
+    simp [h]
+  | abs Γ x e τ₁ τ₂ he ih =>
+    constructor
+    apply ih
+    intro y hy
+    simp [Finmap.insert]
+    simp [Finmap.insert] at hy
+    split_ifs with h
+    · rfl
+    · apply hΓ
+      simp [hy.resolve_left h]
+  | app Γ e₁ e₂ τ₁ τ₂ he₁ he₂ ih₁ ih₂ =>
+    constructor
+    · apply ih₁
+      exact hΓ
+    · apply ih₂
+      exact hΓ
+  | set Γ x e τ hτ he ih =>
+    constructor
+    · rw [← hΓ]
+      · exact hτ
+      apply (Γ.mem_support_is_some x).mpr
+      exact Option.isSome_of_mem hτ
+    · apply ih; exact hΓ
+  | comp Γ e₁ e₂ τ₂ he₁ he₂ ih₁ ih₂ =>
+    constructor
+    · apply ih₁
+      exact hΓ
+    · apply ih₂
+      exact hΓ
+
+
+lemma CExpr.Type.progress Γ c₁ c₂ τ (hΓ: ∀ x, (hμ: x ∈ c₁.μ.dom) → ∃ (hΓ: x ∈ Γ.support),  Γ ⊢ (c₁.μ.get x hμ).expr: Γ.get x hΓ):
+  (Γ ⊢ c₁.e : τ) →
+  (c₁ ⟶ c₂) →
+  ∃ Γ', ((∀ x ∈ Γ.support, Γ x = Γ' x) ∧ Γ' ⊢ c₂.e : τ) := by
+  intro ht he
+  induction he generalizing τ with
+  | var x μ h =>
+    cases ht with | var _ _ _ hΓ' =>
+    simp
+    simp [fvs] at h
+    use Γ
+    constructor
+    · intro x hx
+      rfl
+    · obtain ⟨a, b⟩ :=  hΓ x (by simp [h])
+      simp [Finmap.get, hΓ'] at b
+      exact b
+  | app_l' e₁ e₂ μ h h₁ e₁' μ' h₁' hμ hs ih =>
+    cases ht with | app _ _ _ _ τ₂ ht₁ ht₂ =>
+    simp
+    simp at ih
+    simp at hΓ
+    obtain ⟨Γ', ⟨hμΓ, hτ'⟩⟩ := ih (τ.arrow τ₂) hΓ ht₁
+    use Γ'
+    constructor
+    · exact hμΓ
+    · apply app (τ₂ := τ₂)
+      · exact hτ'
+      · refine weakening _ _ _ _ ?_ ht₂
+        simp
+        exact hμΓ
+  | app_r' v e₂ μ h h₂ e₂' μ' h₂' hμ he₂ ih =>
+    cases ht with | app _ _ _ _ τ₂ hτ₁ hτ₂ =>
+    obtain ⟨Γ', ⟨hμΓ, hτ'⟩⟩ := ih τ₂ hΓ hτ₂
+    use Γ'
+    constructor
+    · exact hμΓ
+    · simp
+      constructor
+      · refine weakening _ _ _ _ ?_ hτ₁
+        exact hμΓ
+      · exact hτ'
+  | app_abs x e v μ h y hy =>
+    cases ht with | app _ _ _ _ τ₂ hτ₁ hτ₂ =>
+    use (Γ.insert y τ₂)
+    constructor
+    · intro x hx
+      simp [Finmap.insert]
+      intro contra
+      sorry
+  | set' x e μ h h₁ e' μ' h' hμ' he ih =>
+    cases ht with
+
+
+
+
+
+
+
+-- lemma CExpr.Type.same_var Γ e τ :
+--   (Γ ⊢ e : τ) → ∀
